model/BTreesModule.v
@@ -13,7 +13,7 @@ Module Type CURSOR_TABLE.
 
  (* Functions of the implementation *)
  Parameter make_cursor: key -> table -> cursor.
- Parameter make_table: cursor -> table.
+ Parameter get_table: cursor -> table.
  Parameter get_key: cursor -> option key.
  Parameter get: cursor -> option V.
  Parameter insert: cursor -> key -> V -> cursor.
@@ -32,8 +32,8 @@ Module Type CURSOR_TABLE.
  (* table-cursor relations *)
  Axiom make_cursor_rel: forall t k,
        abs_rel t (make_cursor k t).
- Axiom make_table_rel: forall t c,
-       abs_rel t c <-> make_table c = t.
+ Axiom get_table_rel: forall t c,
+       abs_rel t c <-> get_table c = t.
  Axiom first_rel: forall t,
        abs_rel t (first_cursor t).
  Axiom last_rel: forall t,
@@ -54,16 +54,17 @@ Module Type CURSOR_TABLE.
        get (last_cursor t) = None.
  Axiom gis: forall k v c,
        cursor_correct c -> key_rel k c ->
-       get (make_cursor k (make_table (insert c k v))) = Some v.
- Axiom gio: forall j k v c t,
-       cursor_correct c -> key_rel k c -> ~ key_rel j c -> abs_rel t c ->
-       get (make_cursor j (make_table (insert c k v))) = get (make_cursor j t).
+       get (make_cursor k (get_table (insert c k v))) = Some v.
+ Axiom gio: forall j k v c,
+       cursor_correct c -> key_rel k c -> ~ key_rel j c ->
+       get (make_cursor j (get_table (insert c k v))) =
+       get (make_cursor j (get_table c)).
 
  (* cursor movement *)
  Axiom next_prev: forall c t,
-       abs_rel t c -> ~ (c = last_cursor t) -> eq_cursor c (prev (next c)).
+       cursor_correct c -> abs_rel t c -> ~ (c = last_cursor t) -> eq_cursor c (prev (next c)).
  Axiom prev_next: forall c t,
-       abs_rel t c -> ~ (c = first_cursor t) -> eq_cursor c (next (prev c)).
+       cursor_correct c -> abs_rel t c -> ~ (c = first_cursor t) -> eq_cursor c (next (prev c)).
  Axiom cursor_order: forall c k1 k2,
        cursor_correct c -> get_key c = Some k1 -> get_key (next c) = Some k2 -> lt_key k1 k2 = true.
 End CURSOR_TABLE.
@@ -81,27 +82,28 @@ Module BT_Table <: CURSOR_TABLE.
  Definition empty_t : table := (BTrees.tl_nil V).
 
  Definition make_cursor (k: key) (m: table) : cursor := BTrees.make_cursor V k m.
- Definition make_table (c : cursor) : table := empty_t. (* complete this *)
+ Definition get_table (c : cursor) : table := BTrees.get_treelist V c.
  Definition get_key (c: cursor) : option key := BTrees.get_key V c.
  Definition get (c: cursor) : option V := BTrees.get V c.
- Definition insert (c: cursor) (k: key) (v: V) : cursor := BTrees.insert V k v c.
+ Definition insert (c: cursor) (k: key) (v: V) : cursor := BTrees.insert V b k v c.
  Definition next (c: cursor) : cursor := BTrees.move_to_next V c.
  Definition prev (c: cursor) : cursor := BTrees.move_to_prev V c.
- Definition first_cursor (m: table) : cursor := ([],[]). (* complete this *)
- Definition last_cursor (m: table) : cursor := ([],[]). (* complete this *)
+ Definition first_cursor (m: table) : cursor := BTrees.first_cursor V m.
+ Definition last_cursor (m: table) : cursor := BTrees.last_cursor V m.
 
- Definition abs_rel (m: table) (c: cursor) : Prop := True. (* complete this *)
- Definition key_rel (k: key) (c: cursor) : Prop := True. (* complete this *)
+ Definition abs_rel (m: table) (c: cursor) : Prop := BTrees.abs_rel V m c.
+ Definition key_rel (k: key) (c: cursor) : Prop := BTrees.key_rel V k c = true.
  Definition eq_cursor c1 c2 : Prop := cursor_elements V c1 = cursor_elements V c2.
- Definition cursor_correct (c: cursor) : Prop := True. (* complete this *)
- Definition table_correct (t: table) : Prop := True. (* complete this *)
+ Definition cursor_correct (c: cursor) : Prop := BTrees.cursor_correct V b c.
+ Definition table_correct (t: table) : Prop :=
+  BTrees.balanced V t /\ BTrees.fanout V b t /\ BTrees.sorted V t.
 
  (* table-cursor relations *)
  Theorem make_cursor_rel: forall t k,
    abs_rel t (make_cursor k t).
- Proof. Admitted. 
- Theorem make_table_rel: forall t c,
-   abs_rel t c <-> make_table c = t.
+ Proof. Admitted.
+ Theorem get_table_rel: forall t c,
+   abs_rel t c <-> get_table c = t.
  Proof. Admitted.
  Theorem first_rel: forall t,
    abs_rel t (first_cursor t).
@@ -130,19 +132,25 @@ Module BT_Table <: CURSOR_TABLE.
  Proof. Admitted.
  Theorem gis: forall k v c,
    cursor_correct c -> key_rel k c ->
-   get (make_cursor k (make_table (insert c k v))) = Some v.
+   get (make_cursor k (get_table (insert c k v))) = Some v.
  Proof. Admitted.
- Theorem gio: forall j k v c t,
-   cursor_correct c -> key_rel k c -> ~ key_rel j c -> abs_rel t c ->
-   get (make_cursor j (make_table (insert c k v))) = get (make_cursor j t).
+ Theorem gio: forall j k v c,
+   cursor_correct c -> key_rel k c -> ~ key_rel j c ->
+   get (make_cursor j (get_table (insert c k v))) =
+   get (make_cursor j (get_table c)).
  Proof. Admitted.
 
  (* cursor movement *)
  Theorem next_prev: forall c t,
-   abs_rel t c -> ~ (c = last_cursor t) -> eq_cursor c (prev (next c)).
- Proof. Admitted.
+   cursor_correct c -> abs_rel t c -> ~ (c = last_cursor t) -> eq_cursor c (prev (next c)).
+ Proof.
+  intros. unfold eq_cursor. destruct (cursor_elements V c) eqn:e. destruct l0.
+  - assert (c = last_cursor t). admit. (* theorem for this *)
+    destruct H1. apply H2.
+  - assert (cursor_elements V (move_to_next V c) = (p::l,l0)). destruct p.
+    admit. Admitted.
  Theorem prev_next: forall c t,
-   abs_rel t c -> ~ (c = first_cursor t) -> eq_cursor c (next (prev c)).
+   cursor_correct c -> abs_rel t c -> ~ (c = first_cursor t) -> eq_cursor c (next (prev c)).
  Proof. Admitted.
  Theorem cursor_order: forall c k1 k2,
    cursor_correct c -> get_key c = Some k1 -> get_key (next c) = Some k2 -> lt_key k1 k2 = true.
